src/checker/Pulse.Reflection.Util.fst
@@ -210,28 +210,28 @@ let mk_stt_ghost_comp_post_equiv (g:R.env) (u:R.universe) (a inames pre post1 po
 
 let mk_total t = R.C_Total t
 let mk_ghost t = R.C_GTotal t
-let binder_of_t_q t q = RT.binder_of_t_q t q
-let binder_of_t_q_s (t:R.term) (q:R.aqualv) (s:RT.pp_name_t) = RT.mk_binder s t q
 let bound_var i : R.term = RT.bound_var i
 let mk_name i : R.term = R.pack_ln (R.Tv_Var (R.pack_namedv (RT.make_namedv i)))
 
-let arrow_dom = (R.term & R.aqualv)
-let mk_arrow (f:arrow_dom) (out:R.term) : R.term =
-  let ty, q = f in
-  R.pack_ln (R.Tv_Arrow (binder_of_t_q ty q) (R.pack_comp (mk_total out)))
-let mk_arrow_with_name (s:RT.pp_name_t) (f:arrow_dom) (out:R.term) : R.term =
-  let ty, q = f in
-  R.pack_ln (R.Tv_Arrow (binder_of_t_q_s ty q s) (R.pack_comp (mk_total out)))
-let mk_ghost_arrow_with_name (s:RT.pp_name_t) (f:arrow_dom) (out:R.term) : R.term =
-  let ty, q = f in
-  R.pack_ln (R.Tv_Arrow (binder_of_t_q_s ty q s) (R.pack_comp (mk_ghost out)))
-let mk_abs ty qual t : R.term = RT.mk_abs ty qual t
-let mk_abs_with_name s ty qual t : R.term =  R.pack_ln (R.Tv_Abs (binder_of_t_q_s ty qual s) t)
-let mk_abs_with_name_and_range s r ty qual t : R.term = 
-  let b = (binder_of_t_q_s ty qual s) in
+let mk_arrow (b:R.binder) (out:R.term) : R.term =
+  R.pack_ln (R.Tv_Arrow b (R.pack_comp (mk_total out)))
+let mk_ghost_arrow (b:R.binder) (out:R.term) : R.term =
+  R.pack_ln (R.Tv_Arrow b (R.pack_comp (mk_ghost out)))
+let mk_abs (b:R.binder) (t:R.term) : R.term =
+  R.pack_ln (R.Tv_Abs b t)
+
+(* Simple versions, just from a type *)
+let mk_arrow0 (ty:R.term) (cod : R.term) : R.term =
+  mk_arrow (RT.mk_simple_binder RT.pp_name_default ty) cod
+let mk_ghost_arrow0 (ty:R.term) (cod : R.term) : R.term =
+  mk_ghost_arrow (RT.mk_simple_binder RT.pp_name_default ty) cod
+let mk_abs0 (ty:R.term) (t:R.term) : R.term =
+  mk_abs (RT.mk_simple_binder RT.pp_name_default ty) t
+
+let mk_abs_with_range (r:Range.range) (b:R.binder) (t:R.term) : R.term =
   let b = RU.binder_set_range b r in
   R.pack_ln (R.Tv_Abs b t)
-  
+
 let mk_erased (u:R.universe) (t:R.term) : R.term =
   let hd = R.pack_ln (R.Tv_UInst (R.pack_fv erased_lid) [u]) in
   R.pack_ln (R.Tv_App hd (t, R.Q_Explicit))
