src/checker/Pulse.Typing.Combinators.fsti
@@ -17,6 +17,7 @@
 module Pulse.Typing.Combinators
 
 module T = FStar.Tactics.V2
+module RT = FStar.Reflection.Typing
 open FStar.List.Tot
 open Pulse.Syntax
 open Pulse.Typing
@@ -24,7 +25,7 @@ open Pulse.Typing
 let st_comp_with_pre (st:st_comp) (pre:term) : st_comp = { st with pre }
 
 let nvar_as_binder (x:nvar) (t:term) : binder =
-  mk_binder_ppname t (fst x)
+  RT.mk_simple_binder (fst x).name t
 
 val slprop_equiv_typing (#g:_) (#t0 #t1:term) (v:slprop_equiv g t0 t1)
   : GTot ((tot_typing g t0 tm_slprop -> tot_typing g t1 tm_slprop) &
